added neon F* extraction

libcrux-intrinsics/src/lib.rs
@@ -1,16 +1,14 @@
-// #[cfg(all(feature = "simd128", not(eurydice), not(hax)))]
-#[cfg(feature = "simd128")]
+#[cfg(all(feature = "simd128", not(eurydice), not(hax)))]
 pub mod arm64;
-// #[cfg(all(feature = "simd256", not(eurydice), not(hax)))]
-#[cfg(feature = "simd256")]
+#[cfg(all(feature = "simd256", not(eurydice), not(hax)))]
 pub mod avx2;
 
-// // When extracting C or F* we only want dummy files here.
-// #[cfg(all(feature = "simd128", any(eurydice, hax)))]
-// pub mod arm64_extract;
-// #[cfg(all(feature = "simd128", any(eurydice, hax)))]
-// pub use arm64_extrat as arm64;
-// #[cfg(all(feature = "simd256", any(eurydice, hax)))]
-// pub mod avx2_extract;
-// #[cfg(all(feature = "simd256", any(eurydice, hax)))]
-// pub use avx2_extract as avx2;
+// When extracting C or F* we only want dummy files here.
+#[cfg(all(feature = "simd128", any(eurydice, hax)))]
+pub mod arm64_extract;
+#[cfg(all(feature = "simd128", any(eurydice, hax)))]
+pub use arm64_extract as arm64;
+#[cfg(all(feature = "simd256", any(eurydice, hax)))]
+pub mod avx2_extract;
+#[cfg(all(feature = "simd256", any(eurydice, hax)))]
+pub use avx2_extract as avx2;
