libcrux-ml-kem/src/mlkem512.rs
@@ -229,6 +229,7 @@ let _ =
     (* This module has implicit dependencies, here we make them explicit. *)
     (* The implicit dependencies arise from typeclasses instances. *)
     let open Libcrux_ml_kem.Vector.Portable in
+    let open Libcrux_ml_kem.Vector.Neon in
     ()"))]
             pub fn encapsulate_unpacked(
                 public_key: &MlKem512PublicKeyUnpacked<$vec>,
