libcrux-ml-kem/src/vector/avx2/serialize.rs
@@ -516,16 +516,14 @@ pub(crate) fn deserialize_10(bytes: &[u8]) -> Vec256 {
 pub(crate) fn serialize_11(vector: Vec256) -> [u8; 22] {
     let mut array = [0i16; 16];
     mm256_storeu_si256_i16(&mut array, vector);
-    let input = portable::from_i16_array(array);
-
-    portable::serialize_11(input)
+    let input = crate::vector::portable::PortableVector::from_i16_array(&array);
+    crate::vector::portable::PortableVector::serialize_11(input)
 }
 
 #[inline(always)]
 pub(crate) fn deserialize_11(bytes: &[u8]) -> Vec256 {
-    let output = portable::deserialize_11(bytes);
-
-    let array = portable::to_i16_array(output);
+    let output = crate::vector::portable::PortableVector::deserialize_11(bytes);
+    let array = crate::vector::portable::PortableVector::to_i16_array(output);
     mm256_loadu_si256_i16(&array)
 }
 
