libcrux-ml-kem/proofs/fstar/extraction/Libcrux_ml_kem.Ind_cca.Multiplexing.fst
@@ -16,7 +16,7 @@ let validate_public_key
   else
     if Libcrux_platform.Platform.simd128_support ()
     then
-      Libcrux_ml_kem.Ind_cca.Instantiations.Portable.validate_public_key v_K
+      Libcrux_ml_kem.Ind_cca.Instantiations.Neon.validate_public_key v_K
         v_RANKED_BYTES_PER_RING_ELEMENT
         v_PUBLIC_KEY_SIZE
         public_key
@@ -42,7 +42,7 @@ let decapsulate
   else
     if Libcrux_platform.Platform.simd128_support ()
     then
-      Libcrux_ml_kem.Ind_cca.Instantiations.Portable.decapsulate v_K v_SECRET_KEY_SIZE
+      Libcrux_ml_kem.Ind_cca.Instantiations.Neon.decapsulate v_K v_SECRET_KEY_SIZE
         v_CPA_SECRET_KEY_SIZE v_PUBLIC_KEY_SIZE v_CIPHERTEXT_SIZE v_T_AS_NTT_ENCODED_SIZE v_C1_SIZE
         v_C2_SIZE v_VECTOR_U_COMPRESSION_FACTOR v_VECTOR_V_COMPRESSION_FACTOR v_C1_BLOCK_SIZE v_ETA1
         v_ETA1_RANDOMNESS_SIZE v_ETA2 v_ETA2_RANDOMNESS_SIZE v_IMPLICIT_REJECTION_HASH_INPUT_SIZE
@@ -69,8 +69,8 @@ let encapsulate
   else
     if Libcrux_platform.Platform.simd128_support ()
     then
-      Libcrux_ml_kem.Ind_cca.Instantiations.Portable.encapsulate v_K v_CIPHERTEXT_SIZE
-        v_PUBLIC_KEY_SIZE v_T_AS_NTT_ENCODED_SIZE v_C1_SIZE v_C2_SIZE v_VECTOR_U_COMPRESSION_FACTOR
+      Libcrux_ml_kem.Ind_cca.Instantiations.Neon.encapsulate v_K v_CIPHERTEXT_SIZE v_PUBLIC_KEY_SIZE
+        v_T_AS_NTT_ENCODED_SIZE v_C1_SIZE v_C2_SIZE v_VECTOR_U_COMPRESSION_FACTOR
         v_VECTOR_V_COMPRESSION_FACTOR v_VECTOR_U_BLOCK_LEN v_ETA1 v_ETA1_RANDOMNESS_SIZE v_ETA2
         v_ETA2_RANDOMNESS_SIZE public_key randomness
     else
@@ -97,7 +97,7 @@ let generate_keypair
   else
     if Libcrux_platform.Platform.simd128_support ()
     then
-      Libcrux_ml_kem.Ind_cca.Instantiations.Portable.generate_keypair v_K
+      Libcrux_ml_kem.Ind_cca.Instantiations.Neon.generate_keypair v_K
         v_CPA_PRIVATE_KEY_SIZE
         v_PRIVATE_KEY_SIZE
         v_PUBLIC_KEY_SIZE
