libcrux-ml-kem/proofs/fstar/extraction/Libcrux_ml_kem.Vector.Avx2.Ntt.fst
@@ -3,177 +3,123 @@ module Libcrux_ml_kem.Vector.Avx2.Ntt
 open Core
 open FStar.Mul
 
-let inv_ntt_layer_1_step (vector: Core.Core_arch.X86.t____m256i) (zeta0 zeta1 zeta2 zeta3: i16) =
-  let lhs:Core.Core_arch.X86.t____m256i = Libcrux_intrinsics.Avx2.mm256_shuffle_epi32 245l vector in
-  let rhs:Core.Core_arch.X86.t____m256i = Libcrux_intrinsics.Avx2.mm256_shuffle_epi32 160l vector in
-  let rhs:Core.Core_arch.X86.t____m256i =
-    Libcrux_intrinsics.Avx2.mm256_mullo_epi16 rhs
-      (Libcrux_intrinsics.Avx2.mm256_set_epi16 (-1s) (-1s) 1s 1s (-1s) (-1s) 1s 1s (-1s) (-1s) 1s 1s
-          (-1s) (-1s) 1s 1s
+let inv_ntt_layer_1_step (vector: u8) (zeta0 zeta1 zeta2 zeta3: i16) =
+  let lhs:u8 = Libcrux_intrinsics.Avx2_extract.mm256_shuffle_epi32 245l vector in
+  let rhs:u8 = Libcrux_intrinsics.Avx2_extract.mm256_shuffle_epi32 160l vector in
+  let rhs:u8 =
+    Libcrux_intrinsics.Avx2_extract.mm256_mullo_epi16 rhs
+      (Libcrux_intrinsics.Avx2_extract.mm256_set_epi16 (-1s) (-1s) 1s 1s (-1s) (-1s) 1s 1s (-1s)
+          (-1s) 1s 1s (-1s) (-1s) 1s 1s
         <:
-        Core.Core_arch.X86.t____m256i)
+        u8)
   in
-  let sum:Core.Core_arch.X86.t____m256i = Libcrux_intrinsics.Avx2.mm256_add_epi16 lhs rhs in
-  let sum_times_zetas:Core.Core_arch.X86.t____m256i =
+  let sum:u8 = Libcrux_intrinsics.Avx2_extract.mm256_add_epi16 lhs rhs in
+  let sum_times_zetas:u8 =
     Libcrux_ml_kem.Vector.Avx2.Arithmetic.montgomery_multiply_by_constants sum
-      (Libcrux_intrinsics.Avx2.mm256_set_epi16 zeta3 zeta3 0s 0s zeta2 zeta2 0s 0s zeta1 zeta1 0s 0s
-          zeta0 zeta0 0s 0s
+      (Libcrux_intrinsics.Avx2_extract.mm256_set_epi16 zeta3 zeta3 0s 0s zeta2 zeta2 0s 0s zeta1
+          zeta1 0s 0s zeta0 zeta0 0s 0s
         <:
-        Core.Core_arch.X86.t____m256i)
+        u8)
   in
-  let sum:Core.Core_arch.X86.t____m256i =
-    Libcrux_ml_kem.Vector.Avx2.Arithmetic.barrett_reduce sum
-  in
-  Libcrux_intrinsics.Avx2.mm256_blend_epi16 204l sum sum_times_zetas
+  let sum:u8 = Libcrux_ml_kem.Vector.Avx2.Arithmetic.barrett_reduce sum in
+  Libcrux_intrinsics.Avx2_extract.mm256_blend_epi16 204l sum sum_times_zetas
 
-let inv_ntt_layer_2_step (vector: Core.Core_arch.X86.t____m256i) (zeta0 zeta1: i16) =
-  let lhs:Core.Core_arch.X86.t____m256i =
-    Libcrux_intrinsics.Avx2.mm256_permute4x64_epi64 245l vector
-  in
-  let rhs:Core.Core_arch.X86.t____m256i =
-    Libcrux_intrinsics.Avx2.mm256_permute4x64_epi64 160l vector
-  in
-  let rhs:Core.Core_arch.X86.t____m256i =
-    Libcrux_intrinsics.Avx2.mm256_mullo_epi16 rhs
-      (Libcrux_intrinsics.Avx2.mm256_set_epi16 (-1s) (-1s) (-1s) (-1s) 1s 1s 1s 1s (-1s) (-1s) (-1s)
-          (-1s) 1s 1s 1s 1s
+let inv_ntt_layer_2_step (vector: u8) (zeta0 zeta1: i16) =
+  let lhs:u8 = Libcrux_intrinsics.Avx2_extract.mm256_permute4x64_epi64 245l vector in
+  let rhs:u8 = Libcrux_intrinsics.Avx2_extract.mm256_permute4x64_epi64 160l vector in
+  let rhs:u8 =
+    Libcrux_intrinsics.Avx2_extract.mm256_mullo_epi16 rhs
+      (Libcrux_intrinsics.Avx2_extract.mm256_set_epi16 (-1s) (-1s) (-1s) (-1s) 1s 1s 1s 1s (-1s)
+          (-1s) (-1s) (-1s) 1s 1s 1s 1s
         <:
-        Core.Core_arch.X86.t____m256i)
+        u8)
   in
-  let sum:Core.Core_arch.X86.t____m256i = Libcrux_intrinsics.Avx2.mm256_add_epi16 lhs rhs in
-  let sum_times_zetas:Core.Core_arch.X86.t____m256i =
+  let sum:u8 = Libcrux_intrinsics.Avx2_extract.mm256_add_epi16 lhs rhs in
+  let sum_times_zetas:u8 =
     Libcrux_ml_kem.Vector.Avx2.Arithmetic.montgomery_multiply_by_constants sum
-      (Libcrux_intrinsics.Avx2.mm256_set_epi16 zeta1 zeta1 zeta1 zeta1 0s 0s 0s 0s zeta0 zeta0 zeta0
-          zeta0 0s 0s 0s 0s
+      (Libcrux_intrinsics.Avx2_extract.mm256_set_epi16 zeta1 zeta1 zeta1 zeta1 0s 0s 0s 0s zeta0
+          zeta0 zeta0 zeta0 0s 0s 0s 0s
         <:
-        Core.Core_arch.X86.t____m256i)
+        u8)
   in
-  Libcrux_intrinsics.Avx2.mm256_blend_epi16 240l sum sum_times_zetas
+  Libcrux_intrinsics.Avx2_extract.mm256_blend_epi16 240l sum sum_times_zetas
 
-let inv_ntt_layer_3_step (vector: Core.Core_arch.X86.t____m256i) (zeta: i16) =
-  let lhs:Core.Core_arch.X86.t____m128i =
-    Libcrux_intrinsics.Avx2.mm256_extracti128_si256 1l vector
-  in
-  let rhs:Core.Core_arch.X86.t____m128i = Libcrux_intrinsics.Avx2.mm256_castsi256_si128 vector in
-  let lower_coefficients:Core.Core_arch.X86.t____m128i =
-    Libcrux_intrinsics.Avx2.mm_add_epi16 lhs rhs
-  in
-  let upper_coefficients:Core.Core_arch.X86.t____m128i =
-    Libcrux_intrinsics.Avx2.mm_sub_epi16 lhs rhs
-  in
-  let upper_coefficients:Core.Core_arch.X86.t____m128i =
+let inv_ntt_layer_3_step (vector: u8) (zeta: i16) =
+  let lhs:u8 = Libcrux_intrinsics.Avx2_extract.mm256_extracti128_si256 1l vector in
+  let rhs:u8 = Libcrux_intrinsics.Avx2_extract.mm256_castsi256_si128 vector in
+  let lower_coefficients:u8 = Libcrux_intrinsics.Avx2_extract.mm_add_epi16 lhs rhs in
+  let upper_coefficients:u8 = Libcrux_intrinsics.Avx2_extract.mm_sub_epi16 lhs rhs in
+  let upper_coefficients:u8 =
     Libcrux_ml_kem.Vector.Avx2.Arithmetic.montgomery_multiply_m128i_by_constants upper_coefficients
-      (Libcrux_intrinsics.Avx2.mm_set1_epi16 zeta <: Core.Core_arch.X86.t____m128i)
+      (Libcrux_intrinsics.Avx2_extract.mm_set1_epi16 zeta <: u8)
   in
-  let combined:Core.Core_arch.X86.t____m256i =
-    Libcrux_intrinsics.Avx2.mm256_castsi128_si256 lower_coefficients
-  in
-  Libcrux_intrinsics.Avx2.mm256_inserti128_si256 1l combined upper_coefficients
+  let combined:u8 = Libcrux_intrinsics.Avx2_extract.mm256_castsi128_si256 lower_coefficients in
+  Libcrux_intrinsics.Avx2_extract.mm256_inserti128_si256 1l combined upper_coefficients
 
-let ntt_layer_1_step (vector: Core.Core_arch.X86.t____m256i) (zeta0 zeta1 zeta2 zeta3: i16) =
-  let zetas:Core.Core_arch.X86.t____m256i =
-    Libcrux_intrinsics.Avx2.mm256_set_epi16 (Core.Ops.Arith.Neg.neg zeta3 <: i16)
+let ntt_layer_1_step (vector: u8) (zeta0 zeta1 zeta2 zeta3: i16) =
+  let zetas:u8 =
+    Libcrux_intrinsics.Avx2_extract.mm256_set_epi16 (Core.Ops.Arith.Neg.neg zeta3 <: i16)
       (Core.Ops.Arith.Neg.neg zeta3 <: i16) zeta3 zeta3 (Core.Ops.Arith.Neg.neg zeta2 <: i16)
       (Core.Ops.Arith.Neg.neg zeta2 <: i16) zeta2 zeta2 (Core.Ops.Arith.Neg.neg zeta1 <: i16)
       (Core.Ops.Arith.Neg.neg zeta1 <: i16) zeta1 zeta1 (Core.Ops.Arith.Neg.neg zeta0 <: i16)
       (Core.Ops.Arith.Neg.neg zeta0 <: i16) zeta0 zeta0
   in
-  let rhs:Core.Core_arch.X86.t____m256i = Libcrux_intrinsics.Avx2.mm256_shuffle_epi32 245l vector in
-  let rhs:Core.Core_arch.X86.t____m256i =
-    Libcrux_ml_kem.Vector.Avx2.Arithmetic.montgomery_multiply_by_constants rhs zetas
-  in
-  let lhs:Core.Core_arch.X86.t____m256i = Libcrux_intrinsics.Avx2.mm256_shuffle_epi32 160l vector in
-  Libcrux_intrinsics.Avx2.mm256_add_epi16 lhs rhs
+  let rhs:u8 = Libcrux_intrinsics.Avx2_extract.mm256_shuffle_epi32 245l vector in
+  let rhs:u8 = Libcrux_ml_kem.Vector.Avx2.Arithmetic.montgomery_multiply_by_constants rhs zetas in
+  let lhs:u8 = Libcrux_intrinsics.Avx2_extract.mm256_shuffle_epi32 160l vector in
+  Libcrux_intrinsics.Avx2_extract.mm256_add_epi16 lhs rhs
 
-let ntt_layer_2_step (vector: Core.Core_arch.X86.t____m256i) (zeta0 zeta1: i16) =
-  let zetas:Core.Core_arch.X86.t____m256i =
-    Libcrux_intrinsics.Avx2.mm256_set_epi16 (Core.Ops.Arith.Neg.neg zeta1 <: i16)
+let ntt_layer_2_step (vector: u8) (zeta0 zeta1: i16) =
+  let zetas:u8 =
+    Libcrux_intrinsics.Avx2_extract.mm256_set_epi16 (Core.Ops.Arith.Neg.neg zeta1 <: i16)
       (Core.Ops.Arith.Neg.neg zeta1 <: i16) (Core.Ops.Arith.Neg.neg zeta1 <: i16)
       (Core.Ops.Arith.Neg.neg zeta1 <: i16) zeta1 zeta1 zeta1 zeta1
       (Core.Ops.Arith.Neg.neg zeta0 <: i16) (Core.Ops.Arith.Neg.neg zeta0 <: i16)
       (Core.Ops.Arith.Neg.neg zeta0 <: i16) (Core.Ops.Arith.Neg.neg zeta0 <: i16) zeta0 zeta0 zeta0
       zeta0
   in
-  let rhs:Core.Core_arch.X86.t____m256i = Libcrux_intrinsics.Avx2.mm256_shuffle_epi32 238l vector in
-  let rhs:Core.Core_arch.X86.t____m256i =
-    Libcrux_ml_kem.Vector.Avx2.Arithmetic.montgomery_multiply_by_constants rhs zetas
-  in
-  let lhs:Core.Core_arch.X86.t____m256i = Libcrux_intrinsics.Avx2.mm256_shuffle_epi32 68l vector in
-  Libcrux_intrinsics.Avx2.mm256_add_epi16 lhs rhs
+  let rhs:u8 = Libcrux_intrinsics.Avx2_extract.mm256_shuffle_epi32 238l vector in
+  let rhs:u8 = Libcrux_ml_kem.Vector.Avx2.Arithmetic.montgomery_multiply_by_constants rhs zetas in
+  let lhs:u8 = Libcrux_intrinsics.Avx2_extract.mm256_shuffle_epi32 68l vector in
+  Libcrux_intrinsics.Avx2_extract.mm256_add_epi16 lhs rhs
 
-let ntt_layer_3_step (vector: Core.Core_arch.X86.t____m256i) (zeta: i16) =
-  let rhs:Core.Core_arch.X86.t____m128i =
-    Libcrux_intrinsics.Avx2.mm256_extracti128_si256 1l vector
-  in
-  let rhs:Core.Core_arch.X86.t____m128i =
+let ntt_layer_3_step (vector: u8) (zeta: i16) =
+  let rhs:u8 = Libcrux_intrinsics.Avx2_extract.mm256_extracti128_si256 1l vector in
+  let rhs:u8 =
     Libcrux_ml_kem.Vector.Avx2.Arithmetic.montgomery_multiply_m128i_by_constants rhs
-      (Libcrux_intrinsics.Avx2.mm_set1_epi16 zeta <: Core.Core_arch.X86.t____m128i)
+      (Libcrux_intrinsics.Avx2_extract.mm_set1_epi16 zeta <: u8)
   in
-  let lhs:Core.Core_arch.X86.t____m128i = Libcrux_intrinsics.Avx2.mm256_castsi256_si128 vector in
-  let lower_coefficients:Core.Core_arch.X86.t____m128i =
-    Libcrux_intrinsics.Avx2.mm_add_epi16 lhs rhs
-  in
-  let upper_coefficients:Core.Core_arch.X86.t____m128i =
-    Libcrux_intrinsics.Avx2.mm_sub_epi16 lhs rhs
-  in
-  let combined:Core.Core_arch.X86.t____m256i =
-    Libcrux_intrinsics.Avx2.mm256_castsi128_si256 lower_coefficients
-  in
-  Libcrux_intrinsics.Avx2.mm256_inserti128_si256 1l combined upper_coefficients
+  let lhs:u8 = Libcrux_intrinsics.Avx2_extract.mm256_castsi256_si128 vector in
+  let lower_coefficients:u8 = Libcrux_intrinsics.Avx2_extract.mm_add_epi16 lhs rhs in
+  let upper_coefficients:u8 = Libcrux_intrinsics.Avx2_extract.mm_sub_epi16 lhs rhs in
+  let combined:u8 = Libcrux_intrinsics.Avx2_extract.mm256_castsi128_si256 lower_coefficients in
+  Libcrux_intrinsics.Avx2_extract.mm256_inserti128_si256 1l combined upper_coefficients
 
-let ntt_multiply (lhs rhs: Core.Core_arch.X86.t____m256i) (zeta0 zeta1 zeta2 zeta3: i16) =
-  let shuffle_with:Core.Core_arch.X86.t____m256i =
-    Libcrux_intrinsics.Avx2.mm256_set_epi8 15y 14y 11y 10y 7y 6y 3y 2y 13y 12y 9y 8y 5y 4y 1y 0y 15y
-      14y 11y 10y 7y 6y 3y 2y 13y 12y 9y 8y 5y 4y 1y 0y
+let ntt_multiply (lhs rhs: u8) (zeta0 zeta1 zeta2 zeta3: i16) =
+  let shuffle_with:u8 =
+    Libcrux_intrinsics.Avx2_extract.mm256_set_epi8 15y 14y 11y 10y 7y 6y 3y 2y 13y 12y 9y 8y 5y 4y
+      1y 0y 15y 14y 11y 10y 7y 6y 3y 2y 13y 12y 9y 8y 5y 4y 1y 0y
   in
-  let lhs_shuffled:Core.Core_arch.X86.t____m256i =
-    Libcrux_intrinsics.Avx2.mm256_shuffle_epi8 lhs shuffle_with
-  in
-  let lhs_shuffled:Core.Core_arch.X86.t____m256i =
-    Libcrux_intrinsics.Avx2.mm256_permute4x64_epi64 216l lhs_shuffled
-  in
-  let lhs_evens:Core.Core_arch.X86.t____m128i =
-    Libcrux_intrinsics.Avx2.mm256_castsi256_si128 lhs_shuffled
-  in
-  let lhs_evens:Core.Core_arch.X86.t____m256i =
-    Libcrux_intrinsics.Avx2.mm256_cvtepi16_epi32 lhs_evens
-  in
-  let lhs_odds:Core.Core_arch.X86.t____m128i =
-    Libcrux_intrinsics.Avx2.mm256_extracti128_si256 1l lhs_shuffled
-  in
-  let lhs_odds:Core.Core_arch.X86.t____m256i =
-    Libcrux_intrinsics.Avx2.mm256_cvtepi16_epi32 lhs_odds
-  in
-  let rhs_shuffled:Core.Core_arch.X86.t____m256i =
-    Libcrux_intrinsics.Avx2.mm256_shuffle_epi8 rhs shuffle_with
-  in
-  let rhs_shuffled:Core.Core_arch.X86.t____m256i =
-    Libcrux_intrinsics.Avx2.mm256_permute4x64_epi64 216l rhs_shuffled
-  in
-  let rhs_evens:Core.Core_arch.X86.t____m128i =
-    Libcrux_intrinsics.Avx2.mm256_castsi256_si128 rhs_shuffled
-  in
-  let rhs_evens:Core.Core_arch.X86.t____m256i =
-    Libcrux_intrinsics.Avx2.mm256_cvtepi16_epi32 rhs_evens
-  in
-  let rhs_odds:Core.Core_arch.X86.t____m128i =
-    Libcrux_intrinsics.Avx2.mm256_extracti128_si256 1l rhs_shuffled
-  in
-  let rhs_odds:Core.Core_arch.X86.t____m256i =
-    Libcrux_intrinsics.Avx2.mm256_cvtepi16_epi32 rhs_odds
-  in
-  let left:Core.Core_arch.X86.t____m256i =
-    Libcrux_intrinsics.Avx2.mm256_mullo_epi32 lhs_evens rhs_evens
-  in
-  let right:Core.Core_arch.X86.t____m256i =
-    Libcrux_intrinsics.Avx2.mm256_mullo_epi32 lhs_odds rhs_odds
-  in
-  let right:Core.Core_arch.X86.t____m256i =
-    Libcrux_ml_kem.Vector.Avx2.Arithmetic.montgomery_reduce_i32s right
-  in
-  let right:Core.Core_arch.X86.t____m256i =
-    Libcrux_intrinsics.Avx2.mm256_mullo_epi32 right
-      (Libcrux_intrinsics.Avx2.mm256_set_epi32 (Core.Ops.Arith.Neg.neg (cast (zeta3 <: i16) <: i32)
+  let lhs_shuffled:u8 = Libcrux_intrinsics.Avx2_extract.mm256_shuffle_epi8 lhs shuffle_with in
+  let lhs_shuffled:u8 = Libcrux_intrinsics.Avx2_extract.mm256_permute4x64_epi64 216l lhs_shuffled in
+  let lhs_evens:u8 = Libcrux_intrinsics.Avx2_extract.mm256_castsi256_si128 lhs_shuffled in
+  let lhs_evens:u8 = Libcrux_intrinsics.Avx2_extract.mm256_cvtepi16_epi32 lhs_evens in
+  let lhs_odds:u8 = Libcrux_intrinsics.Avx2_extract.mm256_extracti128_si256 1l lhs_shuffled in
+  let lhs_odds:u8 = Libcrux_intrinsics.Avx2_extract.mm256_cvtepi16_epi32 lhs_odds in
+  let rhs_shuffled:u8 = Libcrux_intrinsics.Avx2_extract.mm256_shuffle_epi8 rhs shuffle_with in
+  let rhs_shuffled:u8 = Libcrux_intrinsics.Avx2_extract.mm256_permute4x64_epi64 216l rhs_shuffled in
+  let rhs_evens:u8 = Libcrux_intrinsics.Avx2_extract.mm256_castsi256_si128 rhs_shuffled in
+  let rhs_evens:u8 = Libcrux_intrinsics.Avx2_extract.mm256_cvtepi16_epi32 rhs_evens in
+  let rhs_odds:u8 = Libcrux_intrinsics.Avx2_extract.mm256_extracti128_si256 1l rhs_shuffled in
+  let rhs_odds:u8 = Libcrux_intrinsics.Avx2_extract.mm256_cvtepi16_epi32 rhs_odds in
+  let left:u8 = Libcrux_intrinsics.Avx2_extract.mm256_mullo_epi32 lhs_evens rhs_evens in
+  let right:u8 = Libcrux_intrinsics.Avx2_extract.mm256_mullo_epi32 lhs_odds rhs_odds in
+  let right:u8 = Libcrux_ml_kem.Vector.Avx2.Arithmetic.montgomery_reduce_i32s right in
+  let right:u8 =
+    Libcrux_intrinsics.Avx2_extract.mm256_mullo_epi32 right
+      (Libcrux_intrinsics.Avx2_extract.mm256_set_epi32 (Core.Ops.Arith.Neg.neg (cast (zeta3 <: i16)
+                <:
+                i32)
             <:
             i32)
           (cast (zeta3 <: i16) <: i32)
@@ -184,28 +130,24 @@ let ntt_multiply (lhs rhs: Core.Core_arch.X86.t____m256i) (zeta0 zeta1 zeta2 zet
           (Core.Ops.Arith.Neg.neg (cast (zeta0 <: i16) <: i32) <: i32)
           (cast (zeta0 <: i16) <: i32)
         <:
-        Core.Core_arch.X86.t____m256i)
+        u8)
   in
-  let products_left:Core.Core_arch.X86.t____m256i =
-    Libcrux_intrinsics.Avx2.mm256_add_epi32 left right
-  in
-  let products_left:Core.Core_arch.X86.t____m256i =
+  let products_left:u8 = Libcrux_intrinsics.Avx2_extract.mm256_add_epi32 left right in
+  let products_left:u8 =
     Libcrux_ml_kem.Vector.Avx2.Arithmetic.montgomery_reduce_i32s products_left
   in
-  let rhs_adjacent_swapped:Core.Core_arch.X86.t____m256i =
-    Libcrux_intrinsics.Avx2.mm256_shuffle_epi8 rhs
-      (Libcrux_intrinsics.Avx2.mm256_set_epi8 13y 12y 15y 14y 9y 8y 11y 10y 5y 4y 7y 6y 1y 0y 3y 2y
-          13y 12y 15y 14y 9y 8y 11y 10y 5y 4y 7y 6y 1y 0y 3y 2y
+  let rhs_adjacent_swapped:u8 =
+    Libcrux_intrinsics.Avx2_extract.mm256_shuffle_epi8 rhs
+      (Libcrux_intrinsics.Avx2_extract.mm256_set_epi8 13y 12y 15y 14y 9y 8y 11y 10y 5y 4y 7y 6y 1y
+          0y 3y 2y 13y 12y 15y 14y 9y 8y 11y 10y 5y 4y 7y 6y 1y 0y 3y 2y
         <:
-        Core.Core_arch.X86.t____m256i)
+        u8)
   in
-  let products_right:Core.Core_arch.X86.t____m256i =
-    Libcrux_intrinsics.Avx2.mm256_madd_epi16 lhs rhs_adjacent_swapped
+  let products_right:u8 =
+    Libcrux_intrinsics.Avx2_extract.mm256_madd_epi16 lhs rhs_adjacent_swapped
   in
-  let products_right:Core.Core_arch.X86.t____m256i =
+  let products_right:u8 =
     Libcrux_ml_kem.Vector.Avx2.Arithmetic.montgomery_reduce_i32s products_right
   in
-  let products_right:Core.Core_arch.X86.t____m256i =
-    Libcrux_intrinsics.Avx2.mm256_slli_epi32 16l products_right
-  in
-  Libcrux_intrinsics.Avx2.mm256_blend_epi16 170l products_left products_right
+  let products_right:u8 = Libcrux_intrinsics.Avx2_extract.mm256_slli_epi32 16l products_right in
+  Libcrux_intrinsics.Avx2_extract.mm256_blend_epi16 170l products_left products_right
