libcrux-ml-kem/proofs/fstar/extraction/Libcrux_ml_kem.Vector.Avx2.Sampling.fst
@@ -4,14 +4,12 @@ open Core
 open FStar.Mul
 
 let rejection_sample (input: t_Slice u8) (output: t_Slice i16) =
-  let field_modulus:Core.Core_arch.X86.t____m256i =
-    Libcrux_intrinsics.Avx2.mm256_set1_epi16 Libcrux_ml_kem.Vector.Traits.v_FIELD_MODULUS
+  let field_modulus:u8 =
+    Libcrux_intrinsics.Avx2_extract.mm256_set1_epi16 Libcrux_ml_kem.Vector.Traits.v_FIELD_MODULUS
   in
-  let potential_coefficients:Core.Core_arch.X86.t____m256i =
-    Libcrux_ml_kem.Vector.Avx2.Serialize.deserialize_12_ input
-  in
-  let compare_with_field_modulus:Core.Core_arch.X86.t____m256i =
-    Libcrux_intrinsics.Avx2.mm256_cmpgt_epi16 field_modulus potential_coefficients
+  let potential_coefficients:u8 = Libcrux_ml_kem.Vector.Avx2.Serialize.deserialize_12_ input in
+  let compare_with_field_modulus:u8 =
+    Libcrux_intrinsics.Avx2_extract.mm256_cmpgt_epi16 field_modulus potential_coefficients
   in
   let good:t_Array u8 (sz 2) =
     Libcrux_ml_kem.Vector.Avx2.Serialize.serialize_1_ compare_with_field_modulus
@@ -23,16 +21,20 @@ let rejection_sample (input: t_Slice u8) (output: t_Slice i16) =
       <:
       usize ]
   in
-  let lower_shuffles:Core.Core_arch.X86.t____m128i =
-    Libcrux_intrinsics.Avx2.mm_loadu_si128 (Rust_primitives.unsize lower_shuffles <: t_Slice u8)
+  let lower_shuffles:u8 =
+    Libcrux_intrinsics.Avx2_extract.mm_loadu_si128 (Rust_primitives.unsize lower_shuffles
+        <:
+        t_Slice u8)
   in
-  let lower_coefficients:Core.Core_arch.X86.t____m128i =
-    Libcrux_intrinsics.Avx2.mm256_castsi256_si128 potential_coefficients
+  let lower_coefficients:u8 =
+    Libcrux_intrinsics.Avx2_extract.mm256_castsi256_si128 potential_coefficients
   in
-  let lower_coefficients:Core.Core_arch.X86.t____m128i =
-    Libcrux_intrinsics.Avx2.mm_shuffle_epi8 lower_coefficients lower_shuffles
+  let lower_coefficients:u8 =
+    Libcrux_intrinsics.Avx2_extract.mm_shuffle_epi8 lower_coefficients lower_shuffles
   in
-  let output:t_Slice i16 = Libcrux_intrinsics.Avx2.mm_storeu_si128 output lower_coefficients in
+  let output:t_Slice i16 =
+    Libcrux_intrinsics.Avx2_extract.mm_storeu_si128 output lower_coefficients
+  in
   let sampled_count:usize =
     cast (Core.Num.impl__u8__count_ones (good.[ sz 0 ] <: u8) <: u32) <: usize
   in
@@ -43,14 +45,16 @@ let rejection_sample (input: t_Slice u8) (output: t_Slice i16) =
       <:
       usize ]
   in
-  let upper_shuffles:Core.Core_arch.X86.t____m128i =
-    Libcrux_intrinsics.Avx2.mm_loadu_si128 (Rust_primitives.unsize upper_shuffles <: t_Slice u8)
+  let upper_shuffles:u8 =
+    Libcrux_intrinsics.Avx2_extract.mm_loadu_si128 (Rust_primitives.unsize upper_shuffles
+        <:
+        t_Slice u8)
   in
-  let upper_coefficients:Core.Core_arch.X86.t____m128i =
-    Libcrux_intrinsics.Avx2.mm256_extracti128_si256 1l potential_coefficients
+  let upper_coefficients:u8 =
+    Libcrux_intrinsics.Avx2_extract.mm256_extracti128_si256 1l potential_coefficients
   in
-  let upper_coefficients:Core.Core_arch.X86.t____m128i =
-    Libcrux_intrinsics.Avx2.mm_shuffle_epi8 upper_coefficients upper_shuffles
+  let upper_coefficients:u8 =
+    Libcrux_intrinsics.Avx2_extract.mm_shuffle_epi8 upper_coefficients upper_shuffles
   in
   let output:t_Slice i16 =
     Rust_primitives.Hax.Monomorphized_update_at.update_at_range output
@@ -60,7 +64,7 @@ let rejection_sample (input: t_Slice u8) (output: t_Slice i16) =
         }
         <:
         Core.Ops.Range.t_Range usize)
-      (Libcrux_intrinsics.Avx2.mm_storeu_si128 (output.[ {
+      (Libcrux_intrinsics.Avx2_extract.mm_storeu_si128 (output.[ {
                 Core.Ops.Range.f_start = sampled_count;
                 Core.Ops.Range.f_end = sampled_count +! sz 8 <: usize
               }
