libcrux-ml-kem/proofs/fstar/extraction/Libcrux_ml_kem.Vector.Neon.Vector_type.fsti
@@ -1,0 +1,17 @@
+module Libcrux_ml_kem.Vector.Neon.Vector_type
+#set-options "--fuel 0 --ifuel 1 --z3rlimit 15"
+open Core
+open FStar.Mul
+
+type t_SIMD128Vector = {
+  f_low:u8;
+  f_high:u8
+}
+
+val v_ZERO: Prims.unit -> Prims.Pure t_SIMD128Vector Prims.l_True (fun _ -> Prims.l_True)
+
+val from_i16_array (array: t_Slice i16)
+    : Prims.Pure t_SIMD128Vector Prims.l_True (fun _ -> Prims.l_True)
+
+val to_i16_array (v: t_SIMD128Vector)
+    : Prims.Pure (t_Array i16 (sz 16)) Prims.l_True (fun _ -> Prims.l_True)
